[sledge sem] Sketch out translation correctness
Summary:
This is work in progress; many of the cheats aren't true. In particular,
the definition of stuck/complete/partial traces in LLVM and llair don't
quite match up and need some modification. Also, the state relation
isn't strong enough; it will need to include information about registers
used in the expressions of the LLVM register to llair expression
mapping. But the overall shape of the proof is ok and so it can be
used to poke at various local aspects of the translation, such as
individual instructions.

Reviewed By: jberdine

Differential Revision: D17631604

fbshipit-source-id: 743b5d64d

sledge/semantics/llair_propScript.sml
@@ -9,6 +9,7 @@
 
 open HolKernel boolLib bossLib Parse;
 open arithmeticTheory integerTheory integer_wordTheory wordsTheory listTheory;
+open pred_setTheory finite_mapTheory;
 open settingsTheory miscTheory llairTheory;
 
 new_theory "llair_prop";
@@ -152,6 +153,67 @@ Theorem eval_exp_ignores:
   ∀s1 e v s2. s1.locals = s2.locals ⇒ (eval_exp s1 e v ⇔ eval_exp s2 e v)
 Proof
   metis_tac [eval_exp_ignores_lem]
+QED
+
+Definition exp_uses_def:
+  (exp_uses (Var x) = {x}) ∧
+  (exp_uses Nondet = {}) ∧
+  (exp_uses (Label _) = {}) ∧
+  (exp_uses (Splat e1 e2) = exp_uses e1 ∪ exp_uses e2) ∧
+  (exp_uses (Memory e1 e2) = exp_uses e1 ∪ exp_uses e2) ∧
+  (exp_uses (Concat es) = bigunion (set (map exp_uses es))) ∧
+  (exp_uses (Integer _ _) = {}) ∧
+  (exp_uses (Eq e1 e2) = exp_uses e1 ∪ exp_uses e2) ∧
+  (exp_uses (Lt e1 e2) = exp_uses e1 ∪ exp_uses e2) ∧
+  (exp_uses (Ult e1 e2) = exp_uses e1 ∪ exp_uses e2) ∧
+  (exp_uses (Sub _ e1 e2) = exp_uses e1 ∪ exp_uses e2) ∧
+  (exp_uses (Record es) = bigunion (set (map exp_uses es))) ∧
+  (exp_uses (Select e1 e2) = exp_uses e1 ∪ exp_uses e2) ∧
+  (exp_uses (Update e1 e2 e3) = exp_uses e1 ∪ exp_uses e2 ∪ exp_uses e3)
+Termination
+  WF_REL_TAC `measure exp_size` >> rw [] >>
+  Induct_on `es` >> rw [exp_size_def] >> res_tac >> rw []
+End
+
+Theorem eval_exp_ignores_unused_lem:
+  ∀s1 e v.
+    eval_exp s1 e v ⇒
+    ∀s2. DRESTRICT s1.locals (exp_uses e) = DRESTRICT s2.locals (exp_uses e) ⇒
+    eval_exp s2 e v
+Proof
+  ho_match_mp_tac eval_exp_ind >>
+  rw [exp_uses_def] >> simp [Once eval_exp_cases]
+  >- (
+    fs [DRESTRICT_EQ_DRESTRICT, EXTENSION, FDOM_DRESTRICT] >>
+    imp_res_tac FLOOKUP_SUBMAP >>
+    fs [FLOOKUP_DRESTRICT]) >>
+  fs [drestrict_union_eq]
+  >- metis_tac []
+  >- metis_tac []
+  >- (
+    rpt (pop_assum mp_tac) >>
+    qid_spec_tac `vals` >>
+    Induct_on `es` >> rw [] >> Cases_on `vals` >> rw [PULL_EXISTS] >> fs [] >>
+    rw [] >> fs [drestrict_union_eq] >>
+    rename [`v1++flat vs`] >>
+    first_x_assum (qspec_then `vs` mp_tac) >> rw [] >>
+    qexists_tac `v1 :: vals'` >> rw [])
+  >- metis_tac []
+  >- metis_tac []
+  >- metis_tac []
+  >- metis_tac []
+  >- (
+    rpt (pop_assum mp_tac) >>
+    qid_spec_tac `vals` >>
+    Induct_on `es` >> rw [] >> fs [drestrict_union_eq])
+  >- metis_tac []
+  >- metis_tac []
+QED
+
+Theorem eval_exp_ignores_unused:
+  ∀s1 e v s2. DRESTRICT s1.locals (exp_uses e) = DRESTRICT s2.locals (exp_uses e) ⇒ (eval_exp s1 e v ⇔ eval_exp s2 e v)
+Proof
+  metis_tac [eval_exp_ignores_unused_lem]
 QED
 
 export_theory ();
